Merged all into one file, think about split later

Gale_Shapley.thy
@@ -1,5 +1,5 @@
 theory Gale_Shapley
-  imports "HOL-Library.Permutation" List_Ops
+  imports "HOL-Library.Permutation"
 begin
 type_synonym person = "nat"
 type_synonym man = "person"
@@ -7,15 +7,121 @@ type_synonym woman = "person"
 type_synonym pref_matrix = "(person list) list"
 type_synonym matching = "(woman option) list"
 
-lemma in_upt:"x < k \<longleftrightarrow> x \<in> set [0 ..< k]" by simp
-lemma in_perm_upt: "x < k \<longleftrightarrow> (\<exists>A. A <~~> [0 ..< k] \<and> x \<in> set A)" using in_upt perm_refl perm_set_eq by metis
+lemma in_upt:"x < k \<longleftrightarrow> x \<in> set [0 ..< k]" by auto
+lemma in_perm_upt: "x < k \<longleftrightarrow> (\<exists>A. A <~~> [0 ..< k] \<and> x \<in> set A)"
+  using in_upt by (metis perm_refl perm_set_eq)
 
 fun is_perm::"'a list \<Rightarrow> 'a list \<Rightarrow> bool" where "is_perm A B = (mset A = mset B)"
 lemma is_perm:"is_perm A B \<longleftrightarrow> A <~~> B" using mset_eq_perm by auto
 fun is_valid_pref_matrix::"nat \<Rightarrow> pref_matrix \<Rightarrow> bool" where
-"is_valid_pref_matrix N PPrefs = (if length PPrefs \<noteq> N then False else Ball (set PPrefs) (is_perm [0 ..< N]))"
-lemma length_PPrefs:"is_valid_pref_matrix N PPrefs \<Longrightarrow> length PPrefs = N" using is_valid_pref_matrix.simps by metis
-lemma perm_PPref:"\<lbrakk>is_valid_pref_matrix N PPrefs; m < N\<rbrakk> \<Longrightarrow> PPrefs!m <~~> [0 ..< N]"  using is_valid_pref_matrix.simps nth_mem is_perm perm_sym by metis
+"is_valid_pref_matrix N PPrefs = (if length PPrefs \<noteq> N then False 
+                            else Ball (set PPrefs) (is_perm [0 ..< N]))"
+value "is_valid_pref_matrix 2 [[0, 1],[1, 0]]"
+lemma length_PPrefs:"is_valid_pref_matrix N PPrefs \<Longrightarrow> length PPrefs = N"
+  by (metis is_valid_pref_matrix.simps)
+lemma perm_PPref:"\<lbrakk>is_valid_pref_matrix N PPrefs; m < N\<rbrakk> \<Longrightarrow> PPrefs!m <~~> [0 ..< N]"
+  by (metis is_valid_pref_matrix.simps nth_mem is_perm perm_sym)
+
+fun find_idx::"'a \<Rightarrow> 'a list \<Rightarrow> nat option" where
+"find_idx _ [] = None" |
+"find_idx term (x # xs) = (if term = x then Some 0 else
+                          (case find_idx term xs of None \<Rightarrow> None |
+                                                    Some idx \<Rightarrow> Some (Suc idx)))"
+
+lemma find_idx_bound:"find_idx term xs = Some idx \<Longrightarrow> idx < length xs"
+proof (induction xs arbitrary:idx)
+  case Nil
+  thus ?case by simp
+next
+  case (Cons x xs)
+  show ?case
+  proof cases
+    assume "term = x"
+    with Cons.prems show ?case by simp
+  next
+    assume "term \<noteq> x"
+    moreover with Cons.prems obtain idx' where "find_idx term xs = Some idx'" by force
+    ultimately show ?case using Cons by force
+  qed
+qed
+
+lemma find_idx_Some:"term \<in> set xs \<longleftrightarrow> find_idx term xs \<noteq> None"
+proof
+  have "term \<notin> set xs \<Longrightarrow> find_idx term xs = None"
+    apply (induction xs)
+    by auto
+  thus "find_idx term xs \<noteq> None \<Longrightarrow> term \<in> set xs" by meson
+next
+  show "term \<in> set xs \<Longrightarrow> find_idx term xs \<noteq> None"
+    apply (induction xs)
+     apply simp
+    by force
+qed
+
+lemma find_idx_None:"find_idx term xs = None \<longleftrightarrow> term \<notin> set xs" using find_idx_Some by metis 
+
+lemma find_idx_Some_is_first:"\<lbrakk>find_idx term xs = Some idx; idx' < idx\<rbrakk> \<Longrightarrow> xs!idx' \<noteq> term"
+proof (induction xs arbitrary:idx idx')
+  case Nil
+  thus ?case by simp
+next
+  case (Cons x xs)
+  show ?case
+  proof cases
+    assume "term = x"
+    thus ?case using Cons.prems by simp
+  next
+    assume "term \<noteq> x"
+    moreover with Cons.prems(1) obtain idx_1 where idx_1:"find_idx term xs = Some idx_1" by fastforce
+    ultimately have "idx = Suc idx_1" using Cons.prems(1) by fastforce
+    show ?case
+    proof (cases idx')
+      case 0
+      with `term \<noteq> x` show ?thesis by simp
+    next
+      case (Suc idx'_1)
+      with Cons.prems(2) `idx = Suc idx_1` have "idx'_1 < idx_1" by simp
+      with Cons.IH idx_1 have "xs!idx'_1 \<noteq> term" by simp
+      with Suc show ?thesis by simp
+    qed
+  qed
+qed
+
+lemma find_idx_first_is_Some:"\<lbrakk>idx < length xs; \<forall>idx' < idx. xs!idx' \<noteq> term; xs!idx = term\<rbrakk> \<Longrightarrow> find_idx term xs = Some idx"
+proof (induction xs arbitrary: idx)
+  case Nil
+  thus ?case by simp
+next
+  case (Cons x xs)
+  show ?case
+  proof (cases idx)
+    case 0
+    with Cons.prems(3) show ?thesis by force
+  next
+    case (Suc idx_1)
+    thus ?thesis using Cons by fastforce
+  qed
+qed
+
+lemma find_idx:"term \<in> set xs \<Longrightarrow> xs!the(find_idx term xs) = term"
+proof (induction xs)
+  case Nil
+  thus ?case by simp
+next
+  case (Cons x xs)
+  show ?case
+  proof cases
+    assume "term = x"
+    thus ?case by simp
+  next
+    assume "term \<noteq> x"
+    with Cons.prems have prem:"term \<in> set xs" by auto
+    with find_idx_Some have "find_idx term xs \<noteq> None" by metis
+    then obtain idx where idx:"find_idx term xs = Some idx" by blast
+    hence "xs!idx = term" using Cons.IH prem by simp
+    with idx `term \<noteq> x` show ?case by simp
+  qed
+qed
 
 fun findFreeMan::"matching \<Rightarrow> man option" where
 "findFreeMan engagements = find_idx None engagements"
